LambdaGraph/Lemmas.lean
@@ -1,0 +1,54 @@
+import LambdaGraph.Basic
+
+theorem app_closed_iff {p : Env} {f e : Expr} :
+    (f.app e).Closed p ↔ f.Closed p ∧ e.Closed p := by
+  constructor
+  · intro h
+    constructor <;> solve_by_elim [Free.appL, Free.appR]
+  · rintro ⟨hf, he⟩ n (- | -) <;> solve_by_elim
+
+theorem cond_closed_iff {p : Env} {c et ef : Expr} :
+    (c.cond et ef).Closed p ↔ c.Closed p ∧ et.Closed p ∧ ef.Closed p := by
+  constructor
+  · intro h
+    and_intros <;> solve_by_elim [Free.condC, Free.condT, Free.condF]
+  · rintro ⟨hc, het, hef⟩ n (- | - | -) <;> solve_by_elim
+
+theorem value_types_cn {p : Env} {v : Expr} {t : Ty} (h : p ⊢ v : t.cn) :
+    v.Value → ∃ n, v = .fn n
+  | .fn n => by simp
+  | .bool b => nomatch h
+
+theorem value_types_bool {p : Env} {v : Expr} (h : p ⊢ v : .bool) :
+    v.Value → ∃ b, v = .bool b
+  | .fn n => nomatch h
+  | .bool b => by simp
+
+theorem progress (p : Program) (t : Ty) (ht : ⊢ p : t) (hc : p.Closed) :
+    p.expr.Value ∨ ∃ p', p ⇒ p' := by
+  obtain ⟨p, e⟩ := p
+  obtain ⟨htp, hte⟩ := ht
+  simp only [Program.Closed] at *
+  induction hte with
+  | var n hn => exfalso; exact hc n .var
+  | fn n hn => left; constructor
+  | app f e t htf hte ihf ihe =>
+    right
+    obtain ⟨hcf, hce⟩ := app_closed_iff.mp hc
+    rcases ihf hcf with hvf | ⟨p', hp⟩
+    · rcases ihe hce with hve | ⟨p', hp⟩
+      · obtain ⟨n, rfl⟩ := value_types_cn htf hvf
+        constructor
+        constructor
+        · cases htf
+          assumption
+        · exact hve
+      · exact ⟨_, Step.appR _ _ _ _ _ hvf hp⟩
+    · exact ⟨_, Step.appL _ _ _ _ _ hp⟩
+  | bool b => left; constructor
+  | cond c et ef t htc htet htef ihc ihet ihef =>
+    right
+    obtain ⟨hcc, hcet, hcef⟩ := cond_closed_iff.mp hc
+    rcases ihc hcc with hvc | ⟨p', hp⟩
+    · rcases value_types_bool htc hvc with ⟨_ | _, rfl⟩ <;> repeat constructor
+    · exact ⟨_, Step.condC _ _ _ _ _ _ hp⟩
